chkpt plain_insert lemma stmt

proof/cryptoffi.v
@@ -37,30 +37,30 @@ Qed.
 
 (** Hashes. *)
 
-Definition hash_func (data : list w8) : option $ list w8.
+Definition hash_fn (data : list w8) : option $ list w8.
 Proof. Admitted.
 
-Definition hash_inv_func (hash : list w8) : option $ list w8.
+Definition hash_inv_fn (hash : list w8) : option $ list w8.
 Proof. Admitted.
 
-(* [hash_func] and [hash_inv_func] are partial bijections. *)
+(* [hash_fn] and [hash_inv_fn] are partial bijections. *)
 Lemma hash_bij_l data hash :
-  hash_func data = Some hash →
-  hash_inv_func hash = Some data.
+  hash_fn data = Some hash →
+  hash_inv_fn hash = Some data.
 Proof. Admitted.
 
 Lemma hash_bij_r data hash :
-  hash_inv_func hash = Some data →
-  hash_func data = Some hash.
+  hash_inv_fn hash = Some data →
+  hash_fn data = Some hash.
 Proof. Admitted.
 
 Lemma is_hash_len data hash :
-  hash_func data = Some hash →
+  hash_fn data = Some hash →
   Z.of_nat $ length hash = hash_len.
 Proof. Admitted.
 
 Lemma is_hash_len' data hash :
-  hash_inv_func hash = Some data →
+  hash_inv_fn hash = Some data →
   Z.of_nat $ length hash = hash_len.
 Proof.
   intros Hhash.
@@ -105,7 +105,7 @@ Lemma wp_Hasher_Sum sl_b_in hr data b_in :
     sl_b_out hash, RET #sl_b_out;
     "Hown_hr" ∷ own_Hasher hr data ∗
     "Hsl_b_out" ∷ sl_b_out ↦* (b_in ++ hash) ∗
-    "#His_hash" ∷ ⌜hash_func data = Some hash⌝
+    "#His_hash" ∷ ⌜hash_fn data = Some hash⌝
   }}}.
 Proof. Admitted.
 
@@ -155,40 +155,40 @@ Admitted.
   Persistent (is_vrf_proof pk data proof).
 Proof. Admitted.
 
-(* [vrf_func] does not talk about the VRF proof.
+(* [vrf_fn] does not talk about the VRF proof.
 this is convenient because the spec does not rule out multiple proofs
 between the same pk, data, and output. *)
-(* [vrf_func] models "Full Uniqueness". this always holds for ECVRF. *)
-Definition vrf_func (pk : list w8) (data : list w8) : option $ list w8.
+(* [vrf_fn] models "Full Uniqueness". this always holds for ECVRF. *)
+Definition vrf_fn (pk : list w8) (data : list w8) : option $ list w8.
 Proof. Admitted.
 
-(* [vrf_inv_func] models "Full Collision Resistance".
+(* [vrf_inv_fn] models "Full Collision Resistance".
 From the spec, "Full" (as opposed to "Trusted") holds for ECVRF as long
 as the `validate_key` parameter to `ECVRF_verify` is true.
 key validation is done when running `VrfPublicKeyDecode`
 on an adversarially-provided pk. it is represented by [is_vrf_pk].
 in this model, the partial function internalizes valid keys. *)
-Definition vrf_inv_func (pk : list w8) (out : list w8) : option $ list w8.
+Definition vrf_inv_fn (pk : list w8) (out : list w8) : option $ list w8.
 Proof. Admitted.
 
-(* [vrf_func] and [vrf_inv_func] are partial bijections. *)
+(* [vrf_fn] and [vrf_inv_fn] are partial bijections. *)
 Lemma vrf_bij_l pk data out :
-  vrf_func pk data = Some out →
-  vrf_inv_func pk out = Some data.
+  vrf_fn pk data = Some out →
+  vrf_inv_fn pk out = Some data.
 Proof. Admitted.
 
 Lemma vrf_bij_r pk data out :
-  vrf_inv_func pk out = Some data →
-  vrf_func pk data = Some out.
+  vrf_inv_fn pk out = Some data →
+  vrf_fn pk data = Some out.
 Proof. Admitted.
 
 Lemma is_vrf_len pk data out :
-  vrf_func pk data = Some out →
+  vrf_fn pk data = Some out →
   Z.of_nat $ length out = hash_len.
 Proof. Admitted.
 
 Lemma is_vrf_len' pk data out :
-  vrf_inv_func pk out = Some data →
+  vrf_inv_fn pk out = Some data →
   Z.of_nat $ length out = hash_len.
 Proof.
   intros Hvrf.
@@ -220,7 +220,7 @@ Lemma wp_VrfPrivateKey_Prove ptr_sk pk sl_data (data : list w8) d0 :
     "Hsl_out" ∷ sl_out ↦* out ∗
     "Hsl_proof" ∷ sl_proof ↦* proof ∗
     "#His_vrf_proof" ∷ is_vrf_proof pk data proof ∗
-    "#His_vrf_out" ∷ ⌜vrf_func pk data = Some out⌝
+    "#His_vrf_out" ∷ ⌜vrf_fn pk data = Some out⌝
   }}}.
 Proof. Admitted.
 
@@ -235,7 +235,7 @@ Lemma wp_VrfPrivateKey_Evaluate ptr_sk pk sl_data (data : list w8) d0 :
     sl_out (out : list w8), RET #sl_out;
     "Hsl_data" ∷ sl_data ↦*{d0} data ∗
     "Hsl_out" ∷ sl_out ↦* out ∗
-    "#His_vrf_out" ∷ ⌜vrf_func pk data = Some out⌝
+    "#His_vrf_out" ∷ ⌜vrf_fn pk data = Some out⌝
   }}}.
 Proof. Admitted.
 
@@ -257,7 +257,7 @@ Lemma wp_VrfPublicKey_Verify ptr_pk pk sl_data sl_proof (data proof : list w8) d
       | true => ¬ is_vrf_proof pk data proof
       | false =>
         "#His_proof" ∷ is_vrf_proof pk data proof ∗
-        "#His_out" ∷ ⌜vrf_func pk data = Some out⌝
+        "#His_out" ∷ ⌜vrf_fn pk data = Some out⌝
       end
   }}}.
 Proof. Admitted.
